nola/examples/heap_lang/tactics.v
@@ -56,28 +56,28 @@ Ltac reshape_expr e tac :=
   in
   go (@nil ectx_item) (@nil (val * val)) e.
 
-(** The tactic [inv_head_step] performs inversion on hypotheses of the shape
-[head_step]. The tactic will discharge head-reductions starting from values, and
+(** The tactic [inv_base_step] performs inversion on hypotheses of the shape
+[base_step]. The tactic will discharge head-reductions starting from values, and
 simplifies hypothesis related to conversions from and to values, and finite map
 operations. This tactic is slightly ad-hoc and tuned for proving our lifting
 lemmas. *)
-Ltac inv_head_step :=
+Ltac inv_base_step :=
   repeat match goal with
   | _ => progress simplify_map_eq/= (* simplify memory stuff *)
   | H : to_val _ = Some _ |- _ => apply of_to_val in H
-  | H : head_step ?e _ _ _ _ _ |- _ =>
+  | H : base_step ?e _ _ _ _ _ |- _ =>
      try (is_var e; fail 1); (* inversion yields many goals if [e] is a variable
      and should thus better be avoided. *)
      inversion H; subst; clear H
   end.
 
-Create HintDb head_step.
-Global Hint Extern 0 (head_reducible _ _) => eexists _, _, _, _; simpl : head_step.
-Global Hint Extern 0 (head_reducible_no_obs _ _) => eexists _, _, _; simpl : head_step.
+Create HintDb base_step.
+Global Hint Extern 0 (base_reducible _ _) => eexists _, _, _, _; simpl : base_step.
+Global Hint Extern 0 (base_reducible_no_obs _ _) => eexists _, _, _; simpl : base_step.
 
 (* [simpl apply] is too stupid, so we need extern hints here. *)
-Global Hint Extern 1 (head_step _ _ _ _ _ _) => econstructor : head_step.
-Global Hint Extern 0 (head_step (CmpXchg _ _ _) _ _ _ _ _) => eapply CmpXchgS : head_step.
-Global Hint Extern 0 (head_step (AllocN _ _) _ _ _ _ _) => apply alloc_fresh : head_step.
-Global Hint Extern 0 (head_step NewProph _ _ _ _ _) => apply new_proph_id_fresh : head_step.
-Global Hint Extern 0 (head_step Ndnat _ _ _ _ _) => apply (NdnatS 0) : head_step.
+Global Hint Extern 1 (base_step _ _ _ _ _ _) => econstructor : base_step.
+Global Hint Extern 0 (base_step (CmpXchg _ _ _) _ _ _ _ _) => eapply CmpXchgS : base_step.
+Global Hint Extern 0 (base_step (AllocN _ _) _ _ _ _ _) => apply alloc_fresh : base_step.
+Global Hint Extern 0 (base_step NewProph _ _ _ _ _) => apply new_proph_id_fresh : base_step.
+Global Hint Extern 0 (base_step Ndnat _ _ _ _ _) => apply (NdnatS 0) : base_step.
